\begin{proof}
From Block-MCC$_{q,p}$ (Definition \ref{def:BMIC}, page \pageref{def:BMIC}) we have:
\begin{equation*}
\begin{aligned}
\forall (q , p) \in \mathbb{R}^2_{>0}, \qquad
M_{q,p}\myparanthese{\myPhi} 
\myeq \max_{k,k' \neq k} \frac{d_{k}^{-\frac1p} \, d_{k'}^{\frac1q}}{d_{max}} \mynorm{\myPhi^\dagger\mybracket{k} \myPhi \mybracket{k'}}_{q \to p}.
\end{aligned}
\end{equation*}
Next, considering the relationship between the $\ell_{1 \to 1}$ and $\ell_{1 \to 2}$, and also $\ell_{1 \to 2}$ and $\ell_{1 \to \infty}$ operator-norms, which are presented in general in Property \ref{prp:OperatorProperties} ($\ell_{q {\to} p}$ operator-norm properties) and for certain ($q,p$) pairs in table \ref{table:OperatorNormRelations}, the proof is straightforward, as follows:
\begin{equation*}
\begin{aligned}
M_{1,1}\myparanthese{\myPhi} 
&\myeq \max_{k,k' \neq k} &&\frac{d_{k}^{-1} \, d_{k'}}{d_{max}} \mynorm{\myPhi^\dagger\mybracket{k} \myPhi \mybracket{k'}}_{1 \to 1} \\
&\leq \max_{k,k' \neq k} &&\frac{d_{k}^{-1} \, d_{k'}}{d_{max}} d_{k}^{\frac12} \mynorm{\myPhi^\dagger\mybracket{k} \myPhi \mybracket{k'}}_{1 \to 2} \\
&= \max_{k,k' \neq k} &&\frac{d_{k}^{-\frac12} \, d_{k'}}{d_{max}} \mynorm{\myPhi^\dagger\mybracket{k} \myPhi \mybracket{k'}}_{1 \to 2} \\
&= M_{1,2}\myparanthese{\myPhi} 
&&\leq \max_{k,k' \neq k} \frac{d_{k}^{-\frac12} \, d_{k'}}{d_{max}} d_{k}^{\frac12} \mynorm{\myPhi^\dagger\mybracket{k} \myPhi \mybracket{k'}}_{1 \to \infty} \\
& &&= \max_{k,k' \neq k} \frac{d_{k'}}{d_{max}} \mynorm{\myPhi^\dagger\mybracket{k} \myPhi \mybracket{k'}}_{1 \to \infty} \\
& &&= M_{1,\infty}\myparanthese{\myPhi}.
\end{aligned}
\end{equation*}

Similarly, for the second inequality taking into account the relationship between the $\ell_{2 \to 2}$ and $\ell_{1 \to 2}$ operator-norms, we have:
\begin{equation*}
\begin{aligned}
M_{2,2}\myparanthese{\myPhi} 
&\myeq \max_{k,k' \neq k} \frac{d_{k}^{-\frac12} \, d_{k'}^{\frac12}}{d_{max}} \mynorm{\myPhi^\dagger\mybracket{k} \myPhi \mybracket{k'}}_{2 \to 2} \\
&\leq \max_{k,k' \neq k} \frac{d_{k}^{-\frac12} \, d_{k'}^{\frac12}}{d_{max}} d_{k'}^{\frac12} \mynorm{\myPhi^\dagger\mybracket{k} \myPhi \mybracket{k'}}_{1 \to 2} \\
&= \max_{k,k' \neq k} \frac{d_{k}^{-\frac12} \, d_{k'}}{d_{max}} \mynorm{\myPhi^\dagger\mybracket{k} \myPhi \mybracket{k'}}_{1 \to 2} \\
&= M_{1,2}\myparanthese{\myPhi}.
\end{aligned}
\end{equation*}

Then, for the third inequality considering the relationship between the $\ell_{2 \to 2}$ and $\ell_{2 \to \infty}$, and also $\ell_{2 \to \infty}$ and $\ell_{1 \to \infty}$ operator-norms, we have:
\begin{equation*}
\begin{aligned}
M_{2,2}\myparanthese{\myPhi} 
&\myeq \max_{k,k' \neq k} &&\frac{d_{k}^{-\frac12} \, d_{k'}^{\frac12}}{d_{max}} \mynorm{\myPhi^\dagger\mybracket{k} \myPhi \mybracket{k'}}_{2 \to 2} \\
&\leq \max_{k,k' \neq k} &&\frac{d_{k}^{-\frac12} \, d_{k'}^{\frac12}}{d_{max}} d_{k}^{\frac12} \mynorm{\myPhi^\dagger\mybracket{k} \myPhi \mybracket{k'}}_{2 \to \infty} \\
&= \max_{k,k' \neq k} &&\frac{d_{k'}^{\frac12}}{d_{max}} \mynorm{\myPhi^\dagger\mybracket{k} \myPhi \mybracket{k'}}_{2 \to \infty} \\
&= M_{2 , \infty}\myparanthese{\myPhi} 
&&\leq \max_{k,k' \neq k} \frac{d_{k'}^{\frac12}}{d_{max}} d_{k'}^{\frac12} \mynorm{\myPhi^\dagger\mybracket{k} \myPhi \mybracket{k'}}_{1 \to \infty} \\
& &&= \max_{k,k' \neq k} \frac{d_{k'}}{d_{max}} \mynorm{\myPhi^\dagger\mybracket{k} \myPhi \mybracket{k'}}_{1 \to \infty} \\
& &&= M_{1,\infty}\myparanthese{\myPhi}.
\end{aligned}
\end{equation*}

Finally, for the last inequality we need to know the relationship between the $\ell_{\infty \to \infty}$ and $\ell_{2 \to \infty}$ operator-norms:
\begin{equation*}
\begin{aligned}
M_{\infty,\infty}\myparanthese{\myPhi} 
&\myeq \max_{k,k' \neq k} \frac{1}{d_{max}} \mynorm{\myPhi^\dagger\mybracket{k} \myPhi \mybracket{k'}}_{\infty \to \infty} \\
&\leq \max_{k,k' \neq k} \frac{1}{d_{max}} d_{k'}^{\frac12} \mynorm{\myPhi^\dagger\mybracket{k} \myPhi \mybracket{k'}}_{2 \to \infty} \\
&= \max_{k,k' \neq k} \frac{d_{k'}^{\frac12}}{d_{max}} \mynorm{\myPhi^\dagger\mybracket{k} \myPhi \mybracket{k'}}_{2 \to \infty} \\
&= M_{2 , \infty}\myparanthese{\myPhi}.
\end{aligned}
\end{equation*}

For the proof of general relationships of figure \ref{fig:BMCC_Inequalities}, utilising the upper-bound of second set of bounds in Property \ref{prp:OperatorProperties} ($\ell_{q {\to} p}$ operator-norm properties), i.e., $\forall \myparanthese{q , p , q' , p'} \ssin \mathbb{R}^4_{>0} , \forall \boldsymbol{A} \ssin \mathbb{R}^{m \stimes n} : \Vert \boldsymbol{A} \Vert_{q \to p} \sleq \max \{1 , m^{1/p \sm 1/{p'}} \} \max \{1 , n^{1/{q'} \sm 1/q} \} \Vert \boldsymbol{A} \Vert_{q' \to p'}$, and for a fixed $p \seq p'$, and $q' \sleq q$, which yields $\Vert \boldsymbol{A} \Vert_{q \to p} \sleq n^{1/{q'} \sm 1/q} \Vert \boldsymbol{A} \Vert_{q' \to p}$, we get the following inequalities:
\begin{equation*}
\begin{aligned}
\forall (q , p , q') \in \mathbb{R}^3_{>0}, q' \leq q, \qquad
M_{q,p}\myparanthese{\myPhi} 
&\myeq \max_{k,k' \neq k} \frac{d_{k}^{-\frac1p} \, d_{k'}^{\frac1q}}{d_{max}} \mynorm{\myPhi^\dagger\mybracket{k} \myPhi \mybracket{k'}}_{q \to p} \\
&\leq \max_{k,k' \neq k} \frac{d_{k}^{-\frac1p} \, d_{k'}^{\frac1q}}{d_{max}} \, d_{k'}^{\frac{1}{q'} - \frac1q} \, \mynorm{\myPhi^\dagger\mybracket{k} \myPhi \mybracket{k'}}_{q' \to p} \\
&= \max_{k,k' \neq k} \frac{d_{k}^{-\frac1p} \, d_{k'}^{\frac{1}{q'}}}{d_{max}} \mynorm{\myPhi^\dagger\mybracket{k} \myPhi \mybracket{k'}}_{q' \to p} \\
&= M_{q',p}\myparanthese{\myPhi}.
\end{aligned}
\end{equation*}
Similarly, using the same upper-bound of Property \ref{prp:OperatorProperties}, this time for a fixed $q \seq q'$, and $p \sleq p'$, which yields $\Vert \boldsymbol{A} \Vert_{q \to p} \sleq m^{1/p \sm 1/{p'}} \Vert \boldsymbol{A} \Vert_{q \to p'}$, we get the following inequalities:
\begin{equation*}
\begin{aligned}
\forall (q , p , p') \in \mathbb{R}^3_{>0}, p \leq p', \qquad
M_{q,p}\myparanthese{\myPhi} 
&\myeq \max_{k,k' \neq k} \frac{d_{k}^{-\frac1p} \, d_{k'}^{\frac1q}}{d_{max}} \mynorm{\myPhi^\dagger\mybracket{k} \myPhi \mybracket{k'}}_{q \to p} \\
&\leq \max_{k,k' \neq k} \frac{d_{k}^{-\frac1p} \, d_{k'}^{\frac1q}}{d_{max}} \, d_{k}^{\frac1p - \frac{1}{p'}} \, \mynorm{\myPhi^\dagger\mybracket{k} \myPhi \mybracket{k'}}_{q \to p'} \\
&= \max_{k,k' \neq k} \frac{d_{k}^{-\frac{1}{p'}} \, d_{k'}^{\frac1q}}{d_{max}} \mynorm{\myPhi^\dagger\mybracket{k} \myPhi \mybracket{k'}}_{q \to p'} \\
&= M_{q,p'}\myparanthese{\myPhi}.
\end{aligned}
\end{equation*}
\end{proof}